Nemonuri/TransitionSystemLike/ProgramGraph/Interleaving.lean
@@ -13,79 +13,336 @@ public import Nemonuri.HasHUnion
 
 @[expose] public section
 
+set_option autoImplicit false
+
 namespace Nemonuri.ProgramGraph
+
+universe uvar_l uval_l uec_l uvar_r uval_r uec_r
 
 open HasHUnion
 
 namespace EvalLike
 
-universe uvar_l uval_l uec_l uvar_r uval_r uec_r
+section LeftEvalAt
+
+variable {EC1 EC2: Type uec_l} {Var1 Var2: Type uvar_l} {Val1 Val2: Type uval_l}
+         [EvalLike EC1 Var1 Val1] [EvalLike EC2 Var2 Val2] [HasHUnion Var1 Var2] [HasHUnion Val1 Val2]
+
+scoped instance {lb: Label} : EvalLike (lb.casesOn EC1 EC2) (LeftTypeAt Var1 Var2 lb) (LeftTypeAt Val1 Val2 lb) where
+  coe := lb.casesOn
+          (motive := fun lb0 => (lb0.casesOn EC1 EC2) → Eval (LeftTypeAt Var1 Var2 lb0) (LeftTypeAt Val1 Val2 lb0))
+          (fun x => x)
+          (fun x => x)
+  coe_injective := by cases lb <;> ( exact EvalLike.coe_injective )
+
+def leftEvalAt (ec1: EC1) (ec2: EC2) (lb: Label) : lb.casesOn EC1 EC2 := lb.casesOn ec1 ec2
+
+end LeftEvalAt
 
 structure IsInterleaving
-  (VarL1 VarL2: Type uvar_l) (ValL1 ValL2: Type uval_l) (EC1 EC2: Type uec_l) [EvalLike EC1 VarL1 ValL1] [EvalLike EC2 VarL2 ValL2]
-  [HasHUnion VarL1 VarL2] [HasHUnion ValL1 ValL2]
-  (op: EC1 → EC2 → (HUnionElemAt VarL1 VarL2) → (HUnionElemAt ValL1 ValL2)) : Prop where
-  diff_fst (x: HDiffElemAt VarL1 VarL2 .fst) (ec1: EC1) (ec2: EC2) :
-    .ofEmbedElem (EmbedElemAt.mapAt VarL1 VarL2 ValL1 ValL2 .fst (ec1: Eval VarL1 ValL1) x.toEmbedElem) = op ec1 ec2 (.ofEmbedElem x.toEmbedElem)
-  diff_snd (x: HDiffElemAt VarL1 VarL2 .snd) (ec1: EC1) (ec2: EC2) :
-    .ofEmbedElem (EmbedElemAt.mapAt VarL1 VarL2 ValL1 ValL2 .snd (ec2: Eval VarL2 ValL2) x.toEmbedElem) = op ec1 ec2 (.ofEmbedElem x.toEmbedElem)
-  inter (x: HInterElemAt VarL1 VarL2) (ec1: EC1) (ec2: EC2) :
-    let rhs := op ec1 ec2 (x.toUnion)
-    (.ofEmbedElem (EmbedElemAt.mapAt VarL1 VarL2 ValL1 ValL2 .fst (ec1: Eval VarL1 ValL1) (x.toEmbedElemAt .fst)) = rhs) ∨
-    (.ofEmbedElem (EmbedElemAt.mapAt VarL1 VarL2 ValL1 ValL2 .snd (ec2: Eval VarL2 ValL2) (x.toEmbedElemAt .snd)) = rhs)
+  (EC1 EC2: Type uec_l) (Var1 Var2: Type uvar_l) (Val1 Val2: Type uval_l) [EvalLike EC1 Var1 Val1] [EvalLike EC2 Var2 Val2]
+  [HasHUnion Var1 Var2] [HasHUnion Val1 Val2]
+  (op: EC1 → EC2 → (HUnionElemAt Var1 Var2) → (HUnionElemAt Val1 Val2)) : Prop where
+  diff (ec1: EC1) (ec2: EC2) (lb: Label) (x: HDiffElemAt Var1 Var2 lb) :
+    embedAt Val1 Val2 lb ((leftEvalAt ec1 ec2 lb: Eval (LeftTypeAt Var1 Var2 lb) (LeftTypeAt Val1 Val2 lb)) x.lift) = (op ec1 ec2 (x.toUnion)).val
+  inter (ec1: EC1) (ec2: EC2) (x: HInterElemAt Var1 Var2) :
+    ∃(lb: Label), embedAt Val1 Val2 lb ((leftEvalAt ec1 ec2 lb: Eval (LeftTypeAt Var1 Var2 lb) (LeftTypeAt Val1 Val2 lb)) (x.liftAt lb)) = (op ec1 ec2 (x.toUnion)).val
 
-structure IsSurjectiveInterleaving
-  (VarL1 VarL2: Type uvar_l) (ValL1 ValL2: Type uval_l) (EC1 EC2: Type uec_l) (ECR: Type uec_r)
-  [HasHUnion VarL1 VarL2] [HasHUnion ValL1 ValL2] [EvalLike EC1 VarL1 ValL1] [EvalLike EC2 VarL2 ValL2] [EvalLike ECR (HUnionElemAt VarL1 VarL2) (HUnionElemAt ValL1 ValL2)]
-  (op: EC1 → EC2 → ECR) : Prop where
-  interleaving: IsInterleaving VarL1 VarL2 ValL1 ValL2 EC1 EC2 (fun ec1 ec2 => op ec1 ec2)
-  surjective: Function.Surjective (Function.uncurry op)
+--#print IsInterleaving
+/-
+  diff_fst (x: HDiffElemAt Var1 Var2 .fst) (ec1: EC1) (ec2: EC2) :
+    embedAt Val1 Val2 .fst ((ec1: Eval Var1 Val1) x.lift) = (op ec1 ec2 (x.toUnion)).val
+  diff_snd (x: HDiffElemAt Var1 Var2 .snd) (ec1: EC1) (ec2: EC2) :
+    embedAt Val1 Val2 .snd ((ec2: Eval Var2 Val2) x.lift) = (op ec1 ec2 (x.toUnion)).val
+  inter (x: HInterElemAt Var1 Var2) (ec1: EC1) (ec2: EC2) :
+    (embedAt Val1 Val2 .fst ((ec1: Eval Var1 Val1) (x.liftAt .fst)) = (op ec1 ec2 (x.toUnion)).val) ∨
+    (embedAt Val1 Val2 .snd ((ec2: Eval Var2 Val2) (x.liftAt .snd)) = (op ec1 ec2 (x.toUnion)).val)
+-/
+    --let rhs := op ec1 ec2 (x.toUnion)
 
-namespace IsSurjectiveInterleaving
+    --(.ofEmbedElem (EmbedElemAt.mapAt Var1 Var2 Val1 Val2 .snd (ec2: Eval Var2 Val2) (x.toEmbedElemAt .snd)) = rhs)
 
-variable {VarL1 VarL2: Type uvar_l} {ValL1 ValL2: Type uval_l} {EC1 EC2: Type uec_l} {ECR: Type uec_r}
+structure IsInterleavingLike
+  (EC1 EC2: Type uec_l) (Var1 Var2: Type uvar_l) (Val1 Val2: Type uval_l) (ECR: Type uec_r)
+  [HasHUnion Var1 Var2] [HasHUnion Val1 Val2] [EvalLike EC1 Var1 Val1] [EvalLike EC2 Var2 Val2] [EvalLike ECR (HUnionElemAt Var1 Var2) (HUnionElemAt Val1 Val2)]
+  (op: EC1 → EC2 → ECR) (inv: ECR → (EC1 × EC2)) (emptyR: ECR) : Prop where
+  interleaving: IsInterleaving EC1 EC2 Var1 Var2 Val1 Val2 (fun ec1 ec2 => op ec1 ec2)
+  right_inverse: Function.RightInverse inv (Function.uncurry op)
+  injective1: Function.Injective (fun ec1 => op ec1 ((inv emptyR).snd))
+  injective2: Function.Injective (fun ec2 => op ((inv emptyR).fst) ec2)
+
+
+namespace IsInterleavingLike
+
+variable {EC1 EC2: Type uec_l} {VarL1 VarL2: Type uvar_l} {ValL1 ValL2: Type uval_l} {ECR: Type uec_r}
          [HasHUnion VarL1 VarL2] [HasHUnion ValL1 ValL2] [EvalLike EC1 VarL1 ValL1] [EvalLike EC2 VarL2 ValL2]
          [EvalLike ECR (HUnionElemAt VarL1 VarL2) (HUnionElemAt ValL1 ValL2)]
+         {op: EC1 → EC2 → ECR} {inv: ECR → (EC1 × EC2)} {emptyR: ECR}
 
-noncomputable def recRightEvalCarrier
-  {op: EC1 → EC2 → ECR} (h: IsSurjectiveInterleaving VarL1 VarL2 ValL1 ValL2 EC1 EC2 ECR op)
+@[elab_as_elim]
+def recRightEval
+  (h: IsInterleavingLike EC1 EC2 VarL1 VarL2 ValL1 ValL2 ECR op inv emptyR)
   {motive: ECR → Sort _}
   (left: (ec1: EC1) → (ec2: EC2) → motive (op ec1 ec2))
   (t: ECR)
   : motive t :=
-  match lm1: Classical.choose (h.surjective t) with
-  | ⟨ec1, ec2⟩ => left ec1 ec2 |> Eq.subst (by
-      have lm2 := Classical.choose_spec (h.surjective t)
-      rewrite [lm1] at lm2
-      simpa using lm2 )
+  let (eq := lm1) ⟨ec1, ec2⟩ := inv t
+  left ec1 ec2 |> Eq.subst (by
+    have lm2 := h.right_inverse.id
+    replace lm1 := congrArg (Function.uncurry op) lm1
+    simp only [funext_iff] at lm2
+    specialize lm2 t
+    simp at lm2
+    rewrite [lm2] at lm1
+    dsimp at lm1
+    exact lm1.symm )
 
-end IsSurjectiveInterleaving
+/-
+@[reducible]
+def toHUnionEval (h: IsInterleavingLike EC1 EC2 VarL1 VarL2 ValL1 ValL2 ECR op inv emptyR) : HasHUnion EC1 EC2 where
+-/
+
+end IsInterleavingLike
 
 
 structure Interleaving
-  (VarL1 VarL2: Type uvar_l) (ValL1 ValL2: Type uval_l) (EC1 EC2: Type uec_l) (ECR: Type uec_r)
+  (EC1 EC2: Type uec_l) (VarL1 VarL2: Type uvar_l) (ValL1 ValL2: Type uval_l) (ECR: Type uec_r)
   [HasHUnion VarL1 VarL2] [HasHUnion ValL1 ValL2] [EvalLike EC1 VarL1 ValL1] [EvalLike EC2 VarL2 ValL2]
   [EvalLike ECR (HUnionElemAt VarL1 VarL2) (HUnionElemAt ValL1 ValL2)] where
   op (ec1: EC1) (ec2: EC2) : ECR
-  valid: IsSurjectiveInterleaving VarL1 VarL2 ValL1 ValL2 EC1 EC2 ECR op
-  --op_interleaving: IsInterleaving VarL1 VarL2 ValL1 ValL2 EC1 EC2 (fun ec1 ec2 => op ec1 ec2)
-  --op_surjective: Function.Surjective (Function.uncurry op)
+  inv (ecr: ECR) : (EC1 × EC2)
+  emptyR : ECR
+  valid: IsInterleavingLike EC1 EC2 VarL1 VarL2 ValL1 ValL2 ECR op inv emptyR
+
 
 
 
 namespace Interleaving
 
-variable {VarL1 VarL2: Type uvar_l} {ValL1 ValL2: Type uval_l} {EC1 EC2: Type uec_l} {ECR: Type uec_r}
-         [HasHUnion VarL1 VarL2] [HasHUnion ValL1 ValL2] [EvalLike EC1 VarL1 ValL1] [EvalLike EC2 VarL2 ValL2]
-         [EvalLike ECR (HUnionElemAt VarL1 VarL2) (HUnionElemAt ValL1 ValL2)]
+variable {EC1 EC2: Type uec_l} {Var1 Var2: Type uvar_l} {Val1 Val2: Type uval_l} {ECR: Type uec_r}
+         [HasHUnion Var1 Var2] [HasHUnion Val1 Val2] [EvalLike EC1 Var1 Val1] [EvalLike EC2 Var2 Val2]
+         [EvalLike ECR (HUnionElemAt Var1 Var2) (HUnionElemAt Val1 Val2)]
+
+theorem inv_injective {il: Interleaving EC1 EC2 Var1 Var2 Val1 Val2 ECR} : Function.Injective (il.inv) :=
+  il.valid.right_inverse.leftInverse.injective
+
+theorem op_uncurry_surjective {il: Interleaving EC1 EC2 Var1 Var2 Val1 Val2 ECR} : Function.Surjective (Function.uncurry il.op) :=
+  il.valid.right_inverse.surjective
+
+theorem op_eq_op_uncurry {il: Interleaving EC1 EC2 Var1 Var2 Val1 Val2 ECR} {ec1: EC1} {ec2: EC2}
+  : il.op ec1 ec2 = Function.uncurry il.op (ec1, ec2) :=
+  Function.uncurry_apply_pair _ _ _ |>.symm
+
+theorem inv_op_eq_self {il: Interleaving EC1 EC2 Var1 Var2 Val1 Val2 ECR} {rv: ECR} : il.op (il.inv rv).fst (il.inv rv).snd = rv := by
+  have lm1 := il.valid.right_inverse.eq rv
+  dsimp [Function.uncurry_def] at lm1
+  exact lm1
+
+theorem inv_op_eq_self_at {il: Interleaving EC1 EC2 Var1 Var2 Val1 Val2 ECR} (rv: ECR) : il.op (il.inv rv).fst (il.inv rv).snd = rv := il.inv_op_eq_self
+
+def emptyAt (il: Interleaving EC1 EC2 Var1 Var2 Val1 Val2 ECR) (lb: Label) : lb.casesOn EC1 EC2 :=
+  lb.projectProd (il.inv il.emptyR)
+
+
+@[defeq]
+theorem inv_emptyR_eq_emptyAt_prod {il: Interleaving EC1 EC2 Var1 Var2 Val1 Val2 ECR}
+  : il.inv il.emptyR = (il.emptyAt .fst, il.emptyAt .snd) :=
+  Label.projectProd_prod_eq.symm
+
+
+theorem emptyAt_prod_op_uncurry_eq_emptyR {il: Interleaving EC1 EC2 Var1 Var2 Val1 Val2 ECR}
+  : Function.uncurry il.op (il.emptyAt .fst, il.emptyAt .snd) = il.emptyR := by
+  dsimp only [← il.inv_emptyR_eq_emptyAt_prod]
+  exact il.valid.right_inverse.eq il.emptyR
+
+theorem emptyAt_op_eq_emptyR {il: Interleaving EC1 EC2 Var1 Var2 Val1 Val2 ECR}
+  : il.op (il.emptyAt .fst) (il.emptyAt .snd) = il.emptyR := by
+  refine Eq.trans ?_ il.emptyAt_prod_op_uncurry_eq_emptyR
+  dsimp
+
+
+theorem emptyAt_fst_self_op_inv_snd_eq_self {il: Interleaving EC1 EC2 Var1 Var2 Val1 Val2 ECR} {ec2: EC2}
+  : (il.inv (il.op (il.emptyAt .fst) ec2)).snd = ec2 := by
+  simp only [← EvalLike.coe_injective.eq_iff, ← DFunLike.coe_injective.eq_iff, funext_iff]
+  intro var
+  have lm1 := il.valid.interleaving
+  rcases lm1 with ⟨lm1, lm2⟩
+/-
+  by_cases lm1: ec2 = il.emptyAt .snd
+  · subst lm1
+    simp [emptyAt_op_eq_emptyR]
+    rfl
+  · simp only [← EvalLike.coe_injective.eq_iff, ← DFunLike.coe_injective.eq_iff, funext_iff] at lm1 ⊢
+    simp at lm1
+    rcases lm1 with ⟨var2_1, lm1⟩
+    intro var2_2
+-/
+/-
+  rw [← EvalLike.coe_injective.eq_iff]
+  rw [← DFunLike.coe_injective.eq_iff]
+-/
+/-
+  have lm1 := il.inv_emptyR_eq_emptyAt_prod
+  simp only [Prod.eq_iff_fst_eq_snd_eq] at lm1
+  rcases lm1 with ⟨lm1, lm2⟩
+  simp only [← lm1]
+  have lm3 := il.valid.injective2
+-/
+
+/-
+  simp only [Prod.eq_iff_fst_eq_snd_eq] at lm1
+  rcases lm1 with ⟨lm1, lm2⟩
+  simp only [← lm1]
+  refine congrArg (Prod.fst) ?_
+  rw [il.inv_injective.eq_iff]
+  refine Eq.trans ?_ il.emptyAt_op_eq_emptyR
+  have lm3 := il.valid.injective2
+  simp only [Prod.eq_iff_fst_eq_snd_eq]
+-/
+/-
+  have lm1 := il.valid.injective2
+  have lm2 := il.inv_injective.comp lm1
+  have lm3 := @lm2.eq_iff
+  simp at lm3
+-/
+  --dsimp [inv_emptyR_eq_emptyAt_prod] at lm2
+
+/-
+theorem op_inv_fst_eq_emptyAt_iff {il: Interleaving EC1 EC2 Var1 Var2 Val1 Val2 ECR} {ec1: EC1} {ec2: EC2}
+  : ((il.inv (il.op ec1 ec2)).fst = il.emptyAt .fst) ↔ (ec1 = il.emptyAt .fst) := by
+-/
+
+/-
+theorem emptyAt_snd_op_inv_eq {il: Interleaving EC1 EC2 Var1 Var2 Val1 Val2 ECR} {ec1: EC1}
+  : il.inv (il.op ec1 (il.emptyAt .snd)) = (ec1, (il.emptyAt .snd)) := by
+  have lm1 := il.valid.injective1 --.eq_iff' --ec1 (il.emptyAt .fst)
+  have lm2 := il.inv_op_eq_self_at il.emptyR
+  have lm3 := lm1.eq_iff' (a := ec1) lm2
+  rewrite [← il.inv_injective.eq_iff] at lm3
+  dsimp [inv_emptyR_eq_emptyAt_prod] at lm3
+-/
+
+  --dsimp [inv_emptyR_eq_emptyAt_prod] at lm1
+  --simp [inv_emptyR_eq_emptyAt_prod] at lm1
+  --rewrite [il.emptyAt_op_eq_emptyR] at lm1
+  --dsimp [Function.Injective] at lm1
+  --rw [op_eq_op_uncurry]
+  --have lm1 := il.op_uncurry_surjective
+  --dsimp [Function.Surjective] at lm1
 
 
 
-theorem op_injective : Function.Injective (@op VarL1 VarL2 ValL1 ValL2 EC1 EC2 ECR _ _ _ _ _) := by
+def embedAt (il: Interleaving EC1 EC2 Var1 Var2 Val1 Val2 ECR) (lb: Label) : (lb.casesOn EC1 EC2) → ECR :=
+  lb.casesOn (motive := fun lb0 => lb0.casesOn EC1 EC2 → ECR)
+             (fun ec1 => il.op ec1 (il.emptyAt .snd))
+             (fun ec2 => il.op (il.emptyAt .fst) ec2)
+
+@[defeq]
+theorem embedAt_fst_eq {il: Interleaving EC1 EC2 Var1 Var2 Val1 Val2 ECR} {ec1: EC1} : (il.embedAt .fst ec1) = il.op ec1 (il.emptyAt .snd) := rfl
+
+@[defeq]
+theorem embedAt_snd_eq {il: Interleaving EC1 EC2 Var1 Var2 Val1 Val2 ECR} {ec2: EC2} : (il.embedAt .snd ec2) = il.op (il.emptyAt .fst) ec2 := rfl
+
+
+theorem embedAt_injective {il: Interleaving EC1 EC2 Var1 Var2 Val1 Val2 ECR} {lb: Label} : Function.Injective (il.embedAt lb) := by
+  cases lb <;> dsimp [embedAt, emptyAt, leftEvalAt]
+  · exact il.valid.injective1
+  · exact il.valid.injective2
+
+theorem embedAt_injective_at {il: Interleaving EC1 EC2 Var1 Var2 Val1 Val2 ECR} (lb: Label) : Function.Injective (il.embedAt lb) := il.embedAt_injective
+
+
+def liftAt (il: Interleaving EC1 EC2 Var1 Var2 Val1 Val2 ECR) (lb: Label) (rv: ECR) : lb.casesOn EC1 EC2 :=
+  lb.projectProd (il.inv rv)
+
+/-
+theorem embedAt_liftAt_eq {il: Interleaving EC1 EC2 Var1 Var2 Val1 Val2 ECR} {lb: Label} (lv: lb.casesOn EC1 EC2)
+  : il.liftAt lb (il.embedAt lb lv) = lv := by
+  cases lb
+  · dsimp [embedAt_fst_eq]
+    dsimp [liftAt, Label.projectProd_prod_fst_eq]
+    by_cases lm1: lv = il.emptyAt .fst
+    · subst lm1
+      simp [emptyAt_op_eq_emptyR]
+      rfl
+    · let x := (lv, il.emptyAt .snd)
+      have lm2 : x.fst = lv := rfl
+      refine Eq.trans ?_ lm2
+      refine congrArg _ ?_
+      clear lm2
+      subst x
+-/
+
+/-
+theorem liftAt_embedAt_eq_self {il: Interleaving EC1 EC2 Var1 Var2 Val1 Val2 ECR} {lb: Label} {rv: ECR} (req: rv ∈ Set.range (il.embedAt lb))
+  : il.embedAt lb (il.liftAt lb rv) = rv := by
+  simp at req
+  rcases req with ⟨ec, req⟩
+  refine Eq.trans ?_ req
+  rw [embedAt_injective.eq_iff]
+  replace req := req.symm
+  subst req
+-/
+/-
+  cases lb
+  · dsimp [liftAt, embedAt, Label.projectProd_prod_fst_eq]
+    refine Eq.trans ?_ il.inv_op_eq_self
+    congr
+    dsimp [emptyAt, Label.projectProd_prod_snd_eq]
+    simp at req
+    rcases req with ⟨ec, req⟩
+    refine congrArg (Prod.snd)
+-/
+
+/-
+
+  dsimp [liftAt]
+-/
+/-
+  have lm1 := il.inv_emptyR_eq_emptyAt_prod
+  simp only [Prod.eq_iff_fst_eq_snd_eq] at lm1
+  rcases lm1 with ⟨lm1, lm2⟩
+  dsimp [liftAt]
+  have lm3 := il.valid.right_inverse.eq
+  have lm4 := lm3 il.emptyR
+  have lm5 := @il.valid.injective1.eq_iff'
+  cases lb
+  · dsimp [Label.projectProd_prod_fst_eq]
+-/
+/-
+    conv =>
+      lhs
+      arg 1
+      arg 2
+      rw [← op_eta]
+-/
+/-
+    have lm1 : Function.Injective (il.embedAt .fst) := il.embedAt_injective
+    have lm2 : Function.Injective (il.embedAt .snd) := il.embedAt_injective
+    dsimp [Function.Injective] at lm1 lm2
+    have lm3 := il.valid.right_inverse.id
+    simp [funext_iff] at lm3
+    have lm4 := lm3 (il.embedAt .fst lv)
+    rw [← (il.embedAt_injective (lb := .fst)).eq_iff]
+    refine Eq.trans ?_ lm4
+    dsimp [embedAt, emptyAt, leftEvalAt, liftAt, Function.uncurry_def]
+    have lm5 := lm3 il.emptyR
+    dsimp [Function.uncurry_def] at lm5
+-/
+    --rw
+    --dsimp [liftAt, leftEvalAt]
+    --dsimp [Function.uncurry_def] at lm1
+    --have lm2 := lm1 il.emptyR
+    --have lm3 := congrArg il.inv lm2
+    --have lm2 := il.valid.injective1
+    --dsimp [Function.Injective] at lm2
+
+/-
+theorem op_injective : Function.Injective (@op EC1 EC2 VarL1 VarL2 ValL1 ValL2 ECR _ _ _ _ _) := by
   rintro ⟨te1, lm1⟩ ⟨te2, lm2⟩ lm3
   simp at lm3 ⊢
   exact lm3
-
+-/
 /-
 structure Eval (il: Interleaving VarL1 VarL2 ValL1 ValL2 EC1 EC2) (ec1: EC1) (ec2: EC2) where
   eval: (HUnionElemAt VarL1 VarL2) → (HUnionElemAt ValL1 ValL2)
@@ -109,7 +366,7 @@ class HasInterleaving (EC1 EC2: Type uec_l) (Var1 Var2: Type uvar_l) (Val1 Val2:
   val: HasHUnion.Bundle.{uval_l, uval_r} Val1 Val2
   R: Type uec_r
   evalLikeR: EvalLike R (HUnionElemAt Var1 Var2) (HUnionElemAt Val1 Val2)
-  interleaving: Interleaving Var1 Var2 Val1 Val2 EC1 EC2 R
+  interleaving: Interleaving EC1 EC2 Var1 Var2 Val1 Val2 R
 
 attribute [reducible, instance] HasInterleaving.var HasInterleaving.val HasInterleaving.evalLikeR
 
@@ -118,7 +375,33 @@ namespace HasInterleaving
 variable {EC1 EC2: Type uec_l} {Var1 Var2: Type uvar_l} {Val1 Val2: Type uval_l} [EvalLike EC1 Var1 Val1] [EvalLike EC2 Var2 Val2]
          [HasInterleaving EC1 EC2 Var1 Var2 Val1 Val2]
 
+def toLiftableEmbedding1 : LiftableEmbedding EC1 (HasInterleaving.R EC1 EC2 Var1 Var2 Val1 Val2) :=
+  let il : Interleaving EC1 EC2 Var1 Var2 Val1 Val2 _ := interleaving
+  let embedding : EC1 ↪ HasInterleaving.R EC1 EC2 Var1 Var2 Val1 Val2 := ⟨il.embedAt .fst, il.embedAt_injective⟩
+  {
+    toEmbedding := embedding
+    lift rv req := (il.inv rv).fst
+    lift_valid lv := by
+      subst embedding
+      dsimp
+      have lm1 := il.valid.injective1
+      have lm2 := il.valid.right_inverse.id
+      simp [funext_iff] at lm2
+      have lm3 := lm2 il.emptyR
+      --have lm3 := @lm1.eq_iff
+      --simp [Function.uncurry_def] at lm3
+  }
 
+/-
+instance : HasHUnion EC1 EC2 where
+  R := HasInterleaving.R EC1 EC2 Var1 Var2 Val1 Val2
+  fst := {
+    toFun := _
+    inj' := _
+    lift := _
+    lift_valid := _
+  }
+-/
 
 end HasInterleaving
 
@@ -138,103 +421,85 @@ def SetOfInterleavingValueDomainAt (sty1: StandardType EC1 Var1 Val1) (sty2: Sta
   HUnionElemAt.setOfHUnion s1 s2
 
 
-
+/-
 def interleave (sty1: StandardType EC1 Var1 Val1) (sty2: StandardType EC2 Var2 Val2) : StandardType (HasInterleaving.R EC1 EC2 Var1 Var2 Val1 Val2) (HUnionElemAt Var1 Var2) (HUnionElemAt Val1 Val2) where
   dom := SetOfInterleavingValueDomainAt sty1 sty2
   valid ec var := by
     have lm1 := sty1.valid
     have lm2 := sty2.valid
-    let il : Interleaving Var1 Var2 Val1 Val2 EC1 EC2 _ := HasInterleaving.interleaving
+    let il : Interleaving EC1 EC2 Var1 Var2 Val1 Val2 _ := HasInterleaving.interleaving
     rcases il with ⟨op, lm3⟩
-    cases ec using (IsSurjectiveInterleaving.recRightEvalCarrier lm3)
+    cases ec using (IsInterleavingLike.recRightEval lm3)
     rename_i ec1 ec2
     specialize lm1 ec1
     specialize lm2 ec2
+    rcases lm3 with ⟨⟨lm3, lm4⟩, lm5, lm6⟩
+    specialize lm3 ec1 ec2
+    specialize lm4 ec1 ec2
     cases var using HUnionElemAt.recDiffInter <;> rename_i x
-    · let x2 := x.toEmbedElem
-      specialize lm1 x2.liftAt
-      dsimp [SetOfInterleavingValueDomainAt, HUnionElemAt.setOfHUnion]
+    · specialize lm3 .fst x
+      specialize lm1 x.lift
+      simp [SetOfInterleavingValueDomainAt, HUnionElemAt.setOfHUnion]
       refine Or.inl ?_
-      simp
-      exists ((ec1: Eval Var1 Val1) x2.liftAt)
+      exists ((ec1: Eval Var1 Val1) x.lift)
       refine ⟨?_, ?_⟩
-      · simp [HUnionElemAt.recLiftDiffAt, DecidableEmbedRange.isInEmbedRangeAt_eq_true_iff, HUnionElemAt.ofEmbedElem]
+      · have lm7 := x.property
+        rewrite [hdiffSetUnivAt_mem_iff_embedRangAt_mem] at lm7
+        dsimp [HUnionElemAt.recLiftDiffAt, HDiffElemAt.toUnion, EmbedElemAt.liftAt]
+        simp [DecidableEmbedRange.isInEmbedRangeAt_eq_true_iff, lm7]
         exact lm1
-      · subst x2
-        rcases lm3 with ⟨⟨lm3_1, lm3_2, lm3_3⟩, lm3_4⟩
-        specialize lm3_1 x ec1 ec2
-        exact lm3_1
-    · let x2 := x.toEmbedElem
-      specialize lm2 x2.liftAt
-      dsimp [SetOfInterleavingValueDomainAt, HUnionElemAt.setOfHUnion]
+      · rw [Subtype.ext_iff, HUnionElemAt.pureAt_val_eq_embedAt]
+        exact lm3
+    · specialize lm3 .snd x
+      specialize lm2 x.lift
+      simp [SetOfInterleavingValueDomainAt, HUnionElemAt.setOfHUnion]
       refine Or.inr ?_
-      simp
-      exists ((ec2: Eval Var2 Val2) x2.liftAt)
+      exists ((ec2: Eval Var2 Val2) x.lift)
       refine ⟨?_, ?_⟩
-      · simp [HUnionElemAt.recLiftDiffAt, DecidableEmbedRange.isInEmbedRangeAt_eq_true_iff, HUnionElemAt.ofEmbedElem]
+      · have lm7 := x.property
+        rewrite [hdiffSetUnivAt_mem_iff_embedRangAt_mem] at lm7
+        dsimp [HUnionElemAt.recLiftDiffAt, HDiffElemAt.toUnion, EmbedElemAt.liftAt]
+        simp [DecidableEmbedRange.isInEmbedRangeAt_eq_true_iff, lm7]
         exact lm2
-      · subst x2
-        rcases lm3 with ⟨⟨lm3_1, lm3_2, lm3_3⟩, lm3_4⟩
-        specialize lm3_2 x ec1 ec2
-        exact lm3_2
-    · rcases lm3 with ⟨⟨lm3_1, lm3_2, lm3_3⟩, lm3_4⟩
-      clear lm3_1 lm3_2 lm3_4
-      specialize lm3_3 x ec1 ec2
-      dsimp at lm3_3
-      let x1 := x.toEmbedElemAt .fst
-      let x2 := x.toEmbedElemAt .snd
-      specialize lm1 x1.liftAt
-      specialize lm2 x2.liftAt
-      rcases lm3_3 with lm3_3 | lm3_3
-      · rw [← lm3_3]
-        dsimp [SetOfInterleavingValueDomainAt, HUnionElemAt.setOfHUnion]
-        simp
-        refine Or.inl ?_
-        exists ((ec1: Eval Var1 Val1) x1.liftAt)
-        refine ⟨?_, ?_⟩
-        · have lm4 := x.property
-          rewrite [hinterSetUnivAt_mem_iff_isInEmbedRangeAt] at lm4
-          replace lm4 := lm4.left
-          simp [HUnionElemAt.recLiftDiffAt, HInterElemAt.toUnion, lm4]
-          subst x1
-          conv at lm1 =>
-            arg 1
-            dsimp [HInterElemAt.toEmbedElemAt, EmbedElemAt.pureAt, HInterElemAt.liftAt]
-            simp [liftAt_embedAt_eq]
-          exact lm1
-        · subst x1
-          dsimp [HInterElemAt.toEmbedElemAt, HInterElemAt.liftAt, HUnionElemAt.pureAt, EmbedElemAt.pureAt, EmbedElemAt.liftAt]
-          simp [liftAt_embedAt_eq]
-          dsimp [EmbedElemAt.mapAt, EmbedElemAt.bindAt, EmbedElemAt.pureAt, EmbedElemAt.liftAt]
-      · rw [← lm3_3]
-        dsimp [SetOfInterleavingValueDomainAt, HUnionElemAt.setOfHUnion]
-        simp
-        refine Or.inr ?_
-        exists ((ec2: Eval Var2 Val2) x2.liftAt)
-        refine ⟨?_, ?_⟩
-        · have lm4 := x.property
-          rewrite [hinterSetUnivAt_mem_iff_isInEmbedRangeAt] at lm4
-          replace lm4 := lm4.right
-          simp [HUnionElemAt.recLiftDiffAt, HInterElemAt.toUnion, lm4]
-          subst x2
-          conv at lm2 =>
-            arg 1
-            dsimp [HInterElemAt.toEmbedElemAt, HUnionElemAt.pureAt, EmbedElemAt.pureAt, HInterElemAt.liftAt]
-            simp [liftAt_embedAt_eq]
-          exact lm2
-        · subst x2
-          dsimp [HInterElemAt.toEmbedElemAt, HInterElemAt.liftAt, HUnionElemAt.pureAt, EmbedElemAt.pureAt, EmbedElemAt.liftAt]
-          simp [liftAt_embedAt_eq]
-          dsimp [EmbedElemAt.mapAt, EmbedElemAt.bindAt, HUnionElemAt.pureAt, EmbedElemAt.pureAt, EmbedElemAt.liftAt]
-
-scoped instance {lb: Label} : EvalLike (lb.casesOn EC1 EC2) (LeftTypeAt Var1 Var2 lb) (LeftTypeAt Val1 Val2 lb) where
-  coe := lb.casesOn
-          (motive := fun lb0 => (lb0.casesOn EC1 EC2) → Eval (LeftTypeAt Var1 Var2 lb0) (LeftTypeAt Val1 Val2 lb0))
-          (fun x => x)
-          (fun x => x)
-  coe_injective := by cases lb <;> ( exact EvalLike.coe_injective )
+      · rw [Subtype.ext_iff, HUnionElemAt.pureAt_val_eq_embedAt]
+        exact lm3
+    · specialize lm4 x
+      specialize lm1 (x.liftAt .fst)
+      specialize lm2 (x.liftAt .snd)
+      rcases lm4 with ⟨lb, lm4⟩
+      simp [SetOfInterleavingValueDomainAt, HUnionElemAt.setOfHUnion, Subtype.ext_iff, HUnionElemAt.pureAt_val_eq_embedAt, ← lm4]
+      have lm7 := x.property
+      rewrite [hinterSetUnivAt_mem_iff_embedRangeAt_mem] at lm7
+      cases lb
+      · refine Or.inl ?_
+        simp [HUnionElemAt.recLiftDiffAt, DecidableEmbedRange.isInEmbedRangeAt_eq_true_iff, HInterElemAt.toUnion, lm7]
+        exists ((ec1: Eval Var1 Val1) (x.liftAt .fst))
+      · refine Or.inr ?_
+        simp [HUnionElemAt.recLiftDiffAt, DecidableEmbedRange.isInEmbedRangeAt_eq_true_iff, HInterElemAt.toUnion, lm7]
+        exists ((ec2: Eval Var2 Val2) (x.liftAt .snd))
 
 
+def invInterleaveAt
+  (x: StandardType (HasInterleaving.R EC1 EC2 Var1 Var2 Val1 Val2) (HUnionElemAt Var1 Var2) (HUnionElemAt Val1 Val2)) (lb: Label)
+  : StandardType (lb.casesOn EC1 EC2) (LeftTypeAt Var1 Var2 lb) (LeftTypeAt Val1 Val2 lb) where
+  dom var := x.dom (.pureAt _ _ lb var) |> (HUnionElemAt.liftSetAt · lb)
+  valid := by
+    let il : Interleaving EC1 EC2 Var1 Var2 Val1 Val2 _ := HasInterleaving.interleaving
+    rcases il with ⟨op, lm1⟩
+    rcases lm1 with ⟨⟨lm1, lm2⟩, lm3, lm4⟩
+    have lm5 := x.valid
+    cases lb
+    · dsimp [LeftTypeAt]
+      intro ec1 lv1
+      simp [HUnionElemAt.liftSetAt]
+      obtain ⟨ec2⟩ := lm3.mp ⟨ec1⟩
+      specialize lm5 (op ec1 ec2) (HUnionElemAt.pureAt _ _ .fst lv1)
+      refine Eq.subst ?_ lm5
+      refine Subtype.ext ?_
+      rw [HUnionElemAt.pureAt_val_eq_embedAt]
+-/
+
+/-
 def invInterleaveAt
   (x: StandardType (HasInterleaving.R EC1 EC2 Var1 Var2 Val1 Val2) (HUnionElemAt Var1 Var2) (HUnionElemAt Val1 Val2)) (lb: Label) [Nonempty (lb.casesOn EC2 EC1)]
   : StandardType (lb.casesOn EC1 EC2) (LeftTypeAt Var1 Var2 lb) (LeftTypeAt Val1 Val2 lb) where
@@ -255,6 +520,8 @@ def invInterleaveAt
       subst ecr
       simp [HUnionElemAt.pureAt, EmbedElemAt.pureAt, HUnionElemAt.ofEmbedElem] at lm3
       rcases lm1 with ⟨lm1_1, lm1_2, lm1_3⟩
+-/
+
 /-
 
     cases lb
